examples/dsls/mini_steel/Pulse.Soundness.Return.fst
@@ -10,10 +10,11 @@ open Pulse.Soundness.Common
 
 module R = FStar.Reflection
 
+module PReflUtil = Pulse.Reflection.Util
 module WT = Pulse.Steel.Wrapper.Typing
 module LN = Pulse.Typing.LN
 
-#push-options "--z3rlimit_factor 30 --fuel 8 --ifuel 8"
+#push-options "--z3rlimit_factor 4 --fuel 8 --ifuel 2"
 let return_soundess
   (#f:stt_env)
   (#g:env)
@@ -29,72 +30,115 @@ let return_soundess
   let rt = elab_term t in
   let re = elab_term e in
   let rpost = elab_term post in
-  let rpost = mk_abs rt R.Q_Explicit rpost in
+  let rpost_abs = mk_abs rt R.Q_Explicit rpost in
   let rt_typing : RT.typing _ rt (R.pack_ln (R.Tv_Type ru)) =
     tot_typing_soundness t_typing in
   let re_typing : RT.typing _ re rt =
     tot_typing_soundness e_typing in
-  let rpost_typing
-    : RT.typing _ rpost
+  let rpost_abs_typing
+    : RT.typing _ rpost_abs
                   (mk_arrow (rt, R.Q_Explicit) vprop_tm) =
     mk_t_abs_tot f g RT.pp_name_default t_typing post_typing in
+  
+  let rx_tm = RT.var_as_term x in
+  let elab_c_pre = RT.open_or_close_term' rpost (RT.OpenWith re) 0 in
+  let pre_eq
+    : RT.equiv (extend_env_l f g)
+               (R.pack_ln (R.Tv_App rpost_abs (re, R.Q_Explicit)))
+               elab_c_pre
+    = RT.EQ_Beta (extend_env_l f g) rt R.Q_Explicit rpost re in  
+  
+  let comp_equiv_noeq (_:unit{use_eq == false})
+    : (match ctag with
+       | STT -> RT.equiv (extend_env_l f g)
+                         (WT.return_stt_noeq_comp ru rt re rpost_abs)
+                         (elab_comp c)
+       | STT_Atomic ->
+         RT.equiv (extend_env_l f g)
+                  (WT.return_stt_atomic_noeq_comp ru rt re rpost_abs)
+                  (elab_comp c)
 
-  // re is ln
-  LN.tot_typing_ln e_typing;
-  elab_ln e (-1);
+       | STT_Ghost ->
+         RT.equiv (extend_env_l f g)
+                  (WT.return_stt_ghost_noeq_comp ru rt re rpost_abs)
+                  (elab_comp c)) =
 
-  // (elab_term post) is (ln 0)
-  RT.well_typed_terms_are_ln _ rpost _ rpost_typing;
-  assert (RT.ln' (elab_term post) 0);
+    
+    match ctag with
+    | STT -> elab_stt_equiv _ c _ _ pre_eq (RT.EQ_Refl _ _)
+    | STT_Atomic -> elab_statomic_equiv _ c _ _ pre_eq (RT.EQ_Refl _ _)
+    | STT_Ghost -> elab_stghost_equiv _ c _ _ pre_eq (RT.EQ_Refl _ _)  in
 
-  assume (ctag == STT /\ use_eq == true);
+  let comp_equiv_eq (_:unit{use_eq == true})
+    : (match ctag with
+       | STT -> RT.equiv (extend_env_l f g)
+                         (WT.return_stt_comp ru rt re rpost_abs x)
+                         (elab_comp c)
+       | STT_Atomic ->
+          RT.equiv (extend_env_l f g)
+                   (WT.return_stt_atomic_comp ru rt re rpost_abs x)
+                   (elab_comp c)
+       | STT_Ghost ->
+          RT.equiv (extend_env_l f g)
+                   (WT.return_stt_ghost_comp ru rt re rpost_abs x)
+                   (elab_comp c)) =
+    
+    assert (elab_term (close_term' (Tm_Star (open_term' post (null_var x) 0)
+                                            (Tm_Pure (mk_eq2_prop u t (null_var x) e))) x 0) ==
+            RT.open_or_close_term' (elab_term (Tm_Star (open_term' post (null_var x) 0)
+                                                       (Tm_Pure (mk_eq2_prop u t (null_var x) e))))
+                                   (RT.CloseVar x) 0);
+    let elab_c_post =
+      mk_abs rt R.Q_Explicit
+        (RT.open_or_close_term'
+           (mk_star
+              (RT.open_or_close_term' rpost (RT.OpenWith rx_tm) 0)
+              (PReflUtil.mk_pure (PReflUtil.mk_eq2 ru rt rx_tm re))) (RT.CloseVar x) 0) in
 
-  // assert (elab_comp c == mk_stt_comp ru rt (elab_term (open_term' post e 0))
-  //                          (RT.mk_abs rt R.Q_Explicit (elab_term (Tm_Star post (Tm_Pure (mk_eq2_prop u t (null_bvar 0) e))))));
+    let post_body_eq
+      : RT.equiv (extend_env_l f g)
+                 (mk_star
+                    (R.pack_ln (R.Tv_App rpost_abs (rx_tm, R.Q_Explicit)))
+                    (PReflUtil.mk_pure (PReflUtil.mk_eq2 ru rt rx_tm re)))
+                 (mk_star
+                    (RT.open_or_close_term' rpost (RT.OpenWith rx_tm) 0)
+                    (PReflUtil.mk_pure (PReflUtil.mk_eq2 ru rt rx_tm re)))
+      = mk_star_equiv _ _ _ _ _ (RT.EQ_Beta _ rt _ _ _) (RT.EQ_Refl _ _) in
 
-  // assert (RT.mk_abs rt R.Q_Explicit (elab_term (Tm_Star post (Tm_Pure (mk_eq2_prop u t (null_bvar 0) e)))) ==
-  //         WT.return_post_with_eq ru rt re rpost x);
+    let post_eq
+      : RT.equiv (extend_env_l f g)
+                 (WT.return_post_with_eq ru rt re rpost_abs x)
+                 elab_c_post
+      = RT.equiv_abs rt R.Q_Explicit x post_body_eq in
 
-  assume (RT.open_or_close_term' (elab_term post) (RT.OpenWith re) 0 ==
-          R.pack_ln (R.Tv_App (RT.mk_abs rt R.Q_Explicit (elab_term post)) (re, R.Q_Explicit)));
-
-  assert (RT.mk_abs rt R.Q_Explicit (elab_term (Tm_Star post (Tm_Pure (mk_eq2_prop u t (null_bvar 0) e)))) ==
-          WT.return_post_with_eq ru rt re rpost x);
-
-  WT.return_stt_typing x rt_typing re_typing rpost_typing
-
-//elab_term (Tm_Star post (Tm_Pure (mk_eq2_prop u t (null_bvar 0) e))))
- 
-  fun _ -> p `star` 0 == e
-
-  fresh x |- (fun _ -> close ((fun _ -> p) x `star` x == e) x)
-
-  // how does equiv commute with open and close?
-
-
-  // elab_open_commute' post e 0;
-  // // RT.beta_reduction rt R.Q_Explicit (elab_term post) re;
-  // let eq
-  //   : RT.equiv (extend_env_l f g)
-  //      (RT.open_or_close_term' (elab_term post) (RT.OpenWith re) 0)
-  //      (R.pack_ln (R.Tv_App (RT.mk_abs rt R.Q_Explicit (elab_term post)) (re, R.Q_Explicit))) =
-  //   RT.EQ_Beta _ rt R.Q_Explicit (elab_term post) re in
-  // let eq = elab_stt_equiv _ c _ _ eq (RT.EQ_Refl _ _) in
-  // match ctag, use_eq with
-  // | STT, true ->
-  //   let d = WT.return_stt_typing x rt_typing re_typing rpost_typing in
-  //   RT.T_Sub _ _ _ _ d
-  //     (RT.ST_Equiv _ _ _ (RT.EQ_Sym _ _ _ eq))
-  // | _ -> admit ()
-
-  // | STT, false -> 
-  //   WT.return_stt_noeq_typing rt_typing re_typing rpost_typing
-  // | STT_Atomic, true ->
-  //   WT.return_stt_atomic_typing x rt_typing re_typing rpost_typing
-  // | STT_Atomic, false -> 
-  //   WT.return_stt_atomic_noeq_typing rt_typing re_typing rpost_typing
-  // | STT_Ghost, true ->
-  //   WT.return_stt_ghost_typing x rt_typing re_typing rpost_typing
-  // | STT_Ghost, false -> 
-  //   WT.return_stt_ghost_noeq_typing rt_typing re_typing rpost_typing
+    match ctag with
+    | STT ->
+      assert (elab_comp c == mk_stt_comp ru rt elab_c_pre elab_c_post);
+      elab_stt_equiv _ c _ _ pre_eq post_eq
+    | STT_Atomic ->
+      assert (elab_comp c == mk_stt_atomic_comp ru rt emp_inames_tm elab_c_pre elab_c_post);
+      elab_statomic_equiv _ c _ _ pre_eq post_eq
+    | STT_Ghost ->
+      assert (elab_comp c == mk_stt_ghost_comp ru rt emp_inames_tm elab_c_pre elab_c_post);
+      elab_stghost_equiv _ c _ _ pre_eq post_eq
+  in
+  match ctag, use_eq with
+  | STT, true ->
+    let d = WT.return_stt_typing x rt_typing re_typing rpost_abs_typing in
+    RT.T_Sub _ _ _ _ d (RT.ST_Equiv _ _ _ (comp_equiv_eq ()))
+  | STT, false ->
+    let d = WT.return_stt_noeq_typing rt_typing re_typing rpost_abs_typing in
+    RT.T_Sub _ _ _ _ d (RT.ST_Equiv _ _ _ (comp_equiv_noeq ()))
+  | STT_Atomic, true ->
+    let d = WT.return_stt_atomic_typing x rt_typing re_typing rpost_abs_typing in
+    RT.T_Sub _ _ _ _ d (RT.ST_Equiv _ _ _ (comp_equiv_eq ()))
+  | STT_Atomic, false ->
+    let d = WT.return_stt_atomic_noeq_typing rt_typing re_typing rpost_abs_typing in
+    RT.T_Sub _ _ _ _ d (RT.ST_Equiv _ _ _ (comp_equiv_noeq ()))
+  | STT_Ghost, true ->
+    let d = WT.return_stt_ghost_typing x rt_typing re_typing rpost_abs_typing in
+    RT.T_Sub _ _ _ _ d (RT.ST_Equiv _ _ _ (comp_equiv_eq ()))
+  | STT_Ghost, false ->
+    let d = WT.return_stt_ghost_noeq_typing rt_typing re_typing rpost_abs_typing in
+    RT.T_Sub _ _ _ _ d (RT.ST_Equiv _ _ _ (comp_equiv_noeq ()))
 #pop-options
